OS NI proof done modulo some assumptions that will later become declassification

verified/secprop/sec_prop.s.dfy
@@ -87,13 +87,14 @@ predicate os_eqentry(e1:PageDbEntryTyped, e2:PageDbEntryTyped)
 {
     match e1
         case Addrspace(_,_,_,_,_)
-            => e2.Addrspace? && e1.(shatrace := e2.shatrace) == e2 // shatrace is irrelevant
-        case L1PTable(_) => e1 == e2
-        case L2PTable(_) => e1 == e2
+            => e2.Addrspace? && e1.(shatrace := e2.shatrace,
+                measurement := e2.measurement, refcount := e2.refcount ) == e2 
         case Dispatcher(_,_,_,_,_) => e2.Dispatcher? &&
             e2.entered == e1.entered && e2.entrypoint == e1.entrypoint
+        case L1PTable(_) => e1 == e2
+        case L2PTable(_) => e1 == e2
         case DataPage(_) => e2.DataPage?
-        case SparePage => e2.SparePage?
+        case SparePage   => e2.SparePage?
 }
 
 predicate {:opaque} os_eqpdb(d1:PageDb, d2:PageDb)
